\section{Proof of 1D Birkhoff Interpolation for polynomials of degree $2n$
    with Point Interpolation}
\label{sec:cvip_birkhoff_pt}

In this section, we interpolate derivative values on the Chebyshev
nodes with the function value at $0$. For ease of notation,
\emph{in this section only} we will label $f(0) = \hat{f}_{1} = a_{0}$ and
label
%
\begin{equation}
    \hat{f}' = \begin{bmatrix} \hat{f}_{2}' & \cdots & \hat{f}_{n+1}'
        \end{bmatrix}^{*}.
\end{equation}
%
The reason will become clear when we see the simplified nature of the
interpolation coefficients.
Now, from Eq.~\eqref{eq:cvip_idct_fhat_prime}, we know
%
\begin{equation}
    \hat{f}_{k}' = \parens{k-1}a_{k-1} + \eta_{k-1},
\end{equation}
%
We find the MSN solution coefficients to be
%
\begin{align}
    \tilde{a} &= D_{s}^{-1}G^{*}
        \begin{bmatrix} 1 &  & \\ & \Gamma & 0 \end{bmatrix}^{+}
        \begin{bmatrix} \hat{f}_{1} \\ \hat{f}' \end{bmatrix} \nonumber\\
    &= \begin{bmatrix} \hat{f}_{1} \\ \frac{c_{2}^{2}\hat{f}_{2}'}{2-1} \\
        \vdots \\ \frac{c_{n}^{2}\hat{f}_{n}'}{n-1} \\
        \frac{\hat{f}_{n+1}'}{n} \\ \frac{s_{n}^{2}\hat{f}_{n}'}{n-1} \\
        \vdots \\ \frac{s_{2}^{2}\hat{f}_{2}'}{2-1} \\ 0 \end{bmatrix}
        \nonumber\\
    &= \begin{bmatrix} a_{0} \\
        c_{2}^{2}a_{1} \\ \vdots \\
        c_{n}^{2}a_{n-1}  \\
        a_{n} \\
        s_{n}^{2}a_{n-1} \\ \vdots \\
        s_{2}^{2}a_{1} \\ 0 \end{bmatrix}
    + \begin{bmatrix} 0 \\
        \frac{c_{2}^{2}}{2-1}\eta_{1} \\ \vdots \\
        \frac{c_{n}^{2}}{n-1}\eta_{n-1} \\
        \frac{1}{n}\eta_{n} \\
        \frac{s_{n}^{2}}{n-1}\eta_{n-1} \\ \vdots \\
        \frac{s_{2}^{2}}{2-1}\eta_{1} \\ 0
    \end{bmatrix}
        \nonumber\\
    &= \tilde{a}_{1} + \tilde{a}_{2}
\end{align}
%
Here, $\tilde{a}_{1}$ includes the main coefficient terms and $\tilde{a}_{2}$
includes the $\eta_{k}$.
We have
%
\begin{align}
    \tau_{k} &= -\parens{\frac{2n+1-k}{k-1}}\parens{\frac{k}{2n+2-k}}^{s}
        \nonumber\\
    c_{k} &= \frac{1}{\sqrt{1+\tau_{k}^{2}}} \nonumber\\
    s_{k} &= \tau_{k}c_{k} \nonumber\\
    \gamma_{k} &= \parens{k-1}k^{-s}\sqrt{1 + \parens{\frac{2n+1-k}{k-1}}^{2}
        \parens{\frac{k}{2n+2-k}}^{2s}} \quad k\in\braces{2,\cdots,n}
        \nonumber\\
    \gamma_{n+1} &= \frac{n}{\parens{n+1}^{s}}
\end{align}
%
from Eqs.~\eqref{eq:v1_D_2n_Givens_cs_def}
and \eqref{eq:v1_I_2n_Givens_gamma_def} in
Sec.~\ref{sec:CV_D_1D_2n_F2}.

Therefore, we see we have
%
\begin{align}
    \norm{a_{c} - \tilde{a}}_{p,1} &\le \norm{a_{c}-\tilde{a}_{1}}_{p,1}
        + \norm{\tilde{a}_{2}}_{p,1} \nonumber\\
    &\le 2\sum_{k=1}^{n}s_{k}^{2}\abs{a_{k-1}}
        + 2\sum_{k=n+1}^{\infty} k\abs{a_{k}} \nonumber\\
    &\le 2\sqrt{\frac{2}{2s+1}}\frac{\norm{a}_{s}}{n^{s-\frac{1}{2}}}
        + \frac{1}{\sqrt{2s-3}}\frac{\norm{a}_{s}}{n^{s-\frac{3}{2}}},
\end{align}
%
where we use bounds from Eqs.~\eqref{eq:bound_xp_01} and 
\eqref{eq:cvip_approx_coefs_tail_bound}.
Thus, we see
%
\begin{equation}
    \norm{f-p_{n}}_{\infty,[-1,1]}
        \le \frac{C_{s}\norm{a}_{s}}{n^{s-\frac{3}{2}}},
\end{equation}
%
with convergence when $\frac{3}{2} < s \le \sigma$.



We now focus on bounding the condition number $\kappa(L)$.
We see
%
\begin{equation}
    \norm{\begin{bmatrix} 1 & \\ & \Gamma \end{bmatrix}}_{2} = 1
\end{equation}
%
under the restriction $s>\frac{3}{2}$, which is required for convergence.
Similarly, we see
%
\begin{align}
    \norm{\begin{bmatrix} 1 & \\ & \Gamma \end{bmatrix}^{-1}}_{2} 
        &= \gamma_{n+1}^{-1} \nonumber\\
    &= n^{s-1}\parens{1+\frac{1}{n}}^{s} \nonumber\\
    &\le 2n^{s-1}, \quad n\ge \brackets{2^{1/s}-1}^{-1},
\end{align}
%
while we also have $\gamma_{n+1}^{-1} \ge n^{s-1}$.
Therefore, $\kappa(L) = \Theta(n^{s-1})$.



