\section{IDCT Coefficients}
\label{sec:cvip_idct}

We now explicitly work out what coefficients are computed using the IDCT.
We first define
%
\begin{align}
    f_{k} &= f(z_{k}^{n}) \nonumber\\
    f_{k}' &= f'(z_{k}^{n}) \nonumber\\
    \bar{f} &= \begin{bmatrix} f(-1) \\ f(1) \end{bmatrix} \nonumber\\
    \widehat{C} &= \begin{bmatrix} 1 & -1 \\ 1 & 1 \end{bmatrix}.
\end{align}
%
It is clear
%
\begin{align}
    \hat{f}_{k} &= \brackets{C^{-1}f}_{k} \nonumber\\
    &= d_{k}\sum_{j=1}^{n} T_{k-1}(z_{j}^{n})f(z_{j}^{n})
        \nonumber\\
    &= d_{k}\sum_{j=1}^{n}T_{k-1}(z_{j}^{n})\brackets{
        \sum_{\ell=0}^{\infty}a_{\ell}T_{\ell}(z_{j}^{n})} \nonumber\\
    &= d_{k}\sum_{\ell=0}^{\infty} a_{\ell}\brackets{
        \sum_{j=1}^{n}T_{k-1}(z_{j}^{n})T_{\ell}(z_{j}^{n})}.
\end{align}
%
Here, $d_{k}$ is the appropriate constant. From work in
Sec.~\ref{sec:CV_mat}, we find
%
\begin{align}
    \hat{f}_{1} &= \sum_{\ell=0}^{\infty} a_{4\ell n}
            - \sum_{\ell=0}^{\infty} a_{2n+4\ell n} \nonumber\\
    \hat{f}_{k} &= \sum_{\ell=0}^{\infty} \brackets{
            a_{k-1+4\ell n} + a_{4n+1-k+4\ell n}} - \sum_{\ell=0}^{\infty}
        \brackets{a_{2n+1-k+4\ell n} + a_{2n-1+k+4\ell n}} \nonumber\\
    &\quad k\in\braces{2,\cdots,n}.
\end{align}
%
In particular, this becomes
%
\begin{equation}
    \hat{f}_{k} = a_{k-1} + \eps_{k},
    \label{eq:cvip_idct_fhat}
\end{equation}
%
where
%
\begin{align}
    \sum_{k=1}^{n} \abs{\eps_{k}} &\le \sum_{k=n+1}^{\infty} \abs{a_{k}}
        \nonumber\\
    &\le \frac{1}{\sqrt{2s-1}}\frac{\norm{a}_{s}}{n^{s-\frac{1}{2}}}.
    \label{eq:cvip_eps_sum}
\end{align}

Similarly, we also have
%
\begin{align}
    \hat{f}_{k}' &= \brackets{UC^{-1}f'}_{k} \nonumber\\
    &= \sum_{\ell=0}^{\infty} \brackets{
        \parens{k+4\ell n}a_{k+4\ell n} +
        \parens{2n-k+4\ell n}a_{2n-k+4\ell n}} \nonumber\\
        &\quad- \sum_{\ell=0}^{\infty}
        \brackets{\parens{2n+k+4\ell n}a_{2n+k+4\ell n} +
        \parens{4n-k+4\ell n}a_{4n-k+4\ell n}} \nonumber\\
    &\quad k\in\braces{1,\cdots,n-1} \nonumber\\
    \hat{f}_{n}' &= \brackets{UC^{-1}f'}_{n} \nonumber\\
    &= \sum_{\ell=0}^{\infty} \parens{n+4\ell n}a_{n+4\ell n}
        - \sum_{\ell=0}^{\infty} \parens{3n+4\ell n}a_{3n+4\ell n}
\end{align}
%
and
%
\begin{align}
    \widehat{C}^{-1}\bar{f} &=
        \begin{bmatrix} \tilde{f}_{1} \\ \tilde{f}_{2}
            \end{bmatrix} \nonumber\\
        \tilde{f}_{1} &= \sum_{\ell=0}^{\infty} a_{2\ell} \nonumber\\
        \tilde{f}_{2} &= \sum_{\ell=0}^{\infty} a_{2\ell+1}.
\end{align}
%
This gives
%
\begin{equation}
    \hat{f}_{k}' = ka_{k} + \eta_{k}
    \label{eq:cvip_idct_fhat_prime}
\end{equation}
%
with
%
\begin{align}
    \sum_{k=1}^{n} \abs{\eta_{k}} &\le \sum_{k=n+1}^{\infty} k\abs{a_{k}}
        \nonumber\\
    &\le \frac{1}{\sqrt{2s-3}}\frac{\norm{a}_{s}}{n^{s-\frac{3}{2}}}.
    \label{eq:cvip_eta_sum}
\end{align}



